More packing lore

DeBruijnSSA/BinSyntax/Rewrite/Region/Compose/Structural.lean
@@ -1,1 +1,94 @@
-import DeBruijnSSA.BinSyntax.Rewrite.Region.Compose.Structural.Basic
+import DeBruijnSSA.BinSyntax.Rewrite.Region.Compose.Structural.Sum
+import DeBruijnSSA.BinSyntax.Rewrite.Region.Compose.Structural.Product
+import DeBruijnSSA.BinSyntax.Rewrite.Term.Compose.Structural
+
+namespace BinSyntax
+
+variable [Φ: EffInstSet φ (Ty α) ε] [PartialOrder α] [SemilatticeSup ε] [OrderBot ε]
+
+namespace Region
+
+def Eqv.packed {Γ Δ : Ctx α ε} {R : LCtx α} (r : Eqv φ Γ R) : Eqv φ ((Γ.pack, ⊥)::Δ) [R.pack]
+  := r.packed_out.packed_in
+
+def Eqv.unpacked {Γ : Ctx α ε} {R : LCtx α} (r : Eqv φ [(Γ.pack, ⊥)] [R.pack]) (h : Γ.Pure)
+  : Eqv φ Γ R := r.unpacked_out.unpacked_in h
+
+theorem Eqv.unpacked_out_unpacked_in {Γ : Ctx α ε} {R : LCtx α}
+  {r : Eqv φ [(Γ.pack, ⊥)] [R.pack]} {h : Γ.Pure}
+  : (r.unpacked_in h).unpacked_out = r.unpacked_out.unpacked_in h := by
+  simp only [unpacked_in, unpacked_out_let1]
+  induction r using Quotient.inductionOn
+  simp only [Term.Eqv.packE_def', vwk_id_quot, unpacked_out_quot, let1_quot]
+  rfl
+
+theorem Eqv.unpacked_out_packed_in {Γ : Ctx α ε} {R : LCtx α}
+  {r : Eqv φ Γ [R.pack]} : r.packed_in.unpacked_out = r.unpacked_out.packed_in (Δ := Δ) := by
+  simp only [unpacked_out, packed_in, vsubst_lsubst]
+  congr
+  simp only [Subst.Eqv.unpack, unpack_def, InS.unpack, Set.mem_setOf_eq, csubst_quot,
+    Term.Subst.Eqv.unpack, Subst.Eqv.vsubst_quot]
+  congr; ext; simp
+
+theorem Eqv.packed_out_unpacked_in {Γ : Ctx α ε} {R : LCtx α}
+  {r : Eqv φ [(Γ.pack, ⊥)] R} {h : Γ.Pure}
+  : (r.unpacked_in h).packed_out = r.packed_out.unpacked_in h := by
+  apply unpacked_out_injective; simp [unpacked_out_unpacked_in]
+
+theorem Eqv.packed_out_packed_in {Γ : Ctx α ε} {R : LCtx α}
+  {r : Eqv φ Γ R} : r.packed_in.packed_out = r.packed_out.packed_in (Δ := Δ) := by
+  apply unpacked_out_injective; simp [unpacked_out_packed_in]
+
+theorem Eqv.packed_def' {Γ : Ctx α ε} {R : LCtx α}
+  {r : Eqv φ Γ R} : r.packed (Δ := Δ) = r.packed_in.packed_out
+  := by simp [packed, packed_out_packed_in]
+
+theorem Eqv.unpacked_def' {Γ : Ctx α ε} {R : LCtx α}
+  {r : Eqv φ [(Γ.pack, ⊥)] [R.pack]} {h : Γ.Pure}
+  : r.unpacked h = r.unpacked_out.unpacked_in h := by simp [unpacked, unpacked_out_unpacked_in]
+
+theorem Eqv.packed_unpacked {Γ : Ctx α ε} {R : LCtx α}
+  {r : Eqv φ [(Γ.pack, ⊥)] [R.pack]} {h : Γ.Pure} : (r.unpacked h).packed = r
+  := by rw [unpacked, packed_def', packed_in_unpacked_in, packed_out_unpacked_out]
+
+theorem Eqv.unpacked_packed {Γ : Ctx α ε} {R : LCtx α}
+  {r : Eqv φ Γ R} {h : Γ.Pure} : r.packed.unpacked h = r
+  := by rw [unpacked, packed_def', unpacked_out_packed_out, unpacked_in_packed_in]
+
+open Term.Eqv
+
+theorem Eqv.packed_br {Γ : Ctx α ε} {L : LCtx α}
+  {ℓ} {a : Term.Eqv φ Γ (A, ⊥)} {hℓ}
+  : (br (L := L) ℓ a hℓ).packed (Δ := Δ) = ret ((a.packed.wk_res ⟨hℓ.get, by rfl⟩).inj) := by
+  rw [packed, packed_out_br, packed_in_br, Term.Eqv.packed_of_inj, ret]
+  congr
+  induction a using Quotient.inductionOn
+  apply Term.Eqv.eq_of_term_eq; rfl
+
+theorem Eqv.packed_let1 {Γ : Ctx α ε} {R : LCtx α}
+  {a : Term.Eqv φ Γ (A, e)} {r : Eqv φ ((A, ⊥)::Γ) R}
+  : (let1 a r).packed (Δ := Δ)
+  = let1 a.packed (let1 (pair (var 1 (by simp)) (var 0 Ctx.Var.shead)) r.packed) := by
+  rw [packed, packed_out_let1, packed_in_let1, <-packed]
+
+theorem Eqv.packed_let2 {Γ : Ctx α ε} {R : LCtx α}
+  {a : Term.Eqv φ Γ (A.prod B, e)} {r : Eqv φ ((B, ⊥)::(A, ⊥)::Γ) R}
+  : (let2 a r).packed (Δ := Δ)
+  = let2 a.packed (let1
+    (pair (pair (var 2 (by simp)) (var 1 (by simp))) (var 0 Ctx.Var.shead))
+    r.packed) := by
+  rw [packed, packed_out_let2, packed_in_let2, <-packed]
+
+theorem Eqv.packed_case {Γ : Ctx α ε} {R : LCtx α}
+  {a : Term.Eqv φ Γ (A.coprod B, e)} {r : Eqv φ ((A, ⊥)::Γ) R} {s : Eqv φ ((B, ⊥)::Γ) R}
+  : (case a r s).packed (Δ := Δ)
+  = case a.packed
+    (let1 (pair (var 1 (by simp)) (var 0 Ctx.Var.shead)) r.packed)
+    (let1 (pair (var 1 (by simp)) (var 0 Ctx.Var.shead)) s.packed) := by
+  simp only [packed, packed_out_case, packed_in_case]
+
+-- TODO: cfg
+
+end Region
+
+end BinSyntax
