DeBruijnSSA/BinSyntax/Rewrite/Term/Compose/Structural.lean
@@ -1,2 +1,12 @@
 import DeBruijnSSA.BinSyntax.Rewrite.Term.Compose.Structural.Sum
 import DeBruijnSSA.BinSyntax.Rewrite.Term.Compose.Structural.Product
+
+namespace BinSyntax
+
+variable [Φ: EffInstSet φ (Ty α) ε] [PartialOrder α] [SemilatticeSup ε] [OrderBot ε]
+
+namespace Term
+
+theorem Eqv.packed_of_inj
+  {Γ : Ctx α ε} {R : LCtx α} {i : Fin R.length} {a : Eqv φ Γ (R.get i, e)}
+  : a.inj.packed (Δ := Δ) = a.packed.inj := by simp [packed]
