DeBruijnSSA/BinSyntax/Rewrite/Term/Compose/Structural/Sum.lean
@@ -15,7 +15,53 @@ def Eqv.inj
   | [] => i.elim0
   | _::R => by cases i using Fin.cases with | zero => exact a.inr | succ i => exact inl (inj a)
 
--- TODO: pack_inj is just inj (nil)
+@[simp]
+theorem Eqv.inj_quot {Γ : Ctx α ε} {R : LCtx α} {i : Fin R.length} {a : InS φ Γ (R.get i, e)}
+  : Eqv.inj ⟦a⟧ = ⟦Term.InS.inj a⟧ := by
+  induction R generalizing Γ with
+  | nil => exact i.elim0
+  | cons _ _ I =>
+    cases i using Fin.cases with
+    | zero => rfl
+    | succ i =>
+      simp only [inj, I, inl_quot, Fin.cases_succ]
+      apply congrArg
+      ext
+      simp [Term.inj, Term.Wf.inj, -Function.iterate_succ, Function.iterate_succ']
+
+@[simp]
+theorem Eqv.wk_inj {Γ Δ : Ctx α ε} {R : LCtx α} {i : Fin R.length}
+  {a : Eqv φ Δ (R.get i, e)} {ρ : Γ.InS Δ}
+  : a.inj.wk ρ = (a.wk ρ).inj := by
+  induction a using Quotient.inductionOn
+  simp only [inj_quot, wk_quot]
+  congr; ext; simp
+
+@[simp]
+theorem Eqv.wk0_inj {Γ : Ctx α ε} {R : LCtx α} {i : Fin R.length}
+  {a : Eqv φ Γ (R.get i, e)} : a.inj.wk0 (head := head) = (a.wk0).inj := wk_inj
+
+@[simp]
+theorem Eqv.wk1_inj {Γ : Ctx α ε} {R : LCtx α} {i : Fin R.length}
+  {a : Eqv φ (V::Γ) (R.get i, e)} : a.inj.wk1 (inserted := inserted) = (a.wk1).inj := wk_inj
+
+@[simp]
+theorem Eqv.subst_inj {Γ Δ : Ctx α ε} {R : LCtx α} {i : Fin R.length}
+  {a : Eqv φ Δ (R.get i, e)} {σ : Subst.Eqv φ Γ Δ}
+  : a.inj.subst σ = (a.subst σ).inj := by
+  induction a using Quotient.inductionOn
+  induction σ using Quotient.inductionOn
+  simp only [inj_quot, subst_quot]
+  congr; ext; simp
+
+@[simp]
+theorem Eqv.inj_zero {Γ : Ctx α ε} {R : LCtx α}
+  {a : Eqv φ Γ (List.get (A::R) (0 : Fin (R.length + 1)), e)}
+  : a.inj = a.inr := rfl
+
+theorem Eqv.inj_succ {Γ : Ctx α ε} {R : LCtx α} {i : Fin R.length}
+  {a : Eqv φ Γ (List.get (A::R) i.succ, e)}
+  : a.inj = (a.inj (R := R)).inl := rfl
 
 def Eqv.inj_n {Γ : Ctx α ε} (R : LCtx α) (i : Fin R.length) : Eqv φ ((R.get i, ⊥)::Γ) (R.pack, e)
   := match R with
@@ -23,7 +69,7 @@ def Eqv.inj_n {Γ : Ctx α ε} (R : LCtx α) (i : Fin R.length) : Eqv φ ((R.get
   | _::R => i.cases (inr nil) (λi => inl (inj_n R i))
 
 theorem Eqv.inj_n_def {Γ : Ctx α ε} {R : LCtx α} {i : Fin R.length}
-  : Eqv.inj_n (φ := φ) (Γ := Γ) R i = ⟦Term.InS.inj_n R i⟧ := by
+  : Eqv.inj_n (φ := φ) (Γ := Γ) (e := e) R i = ⟦Term.InS.inj_n R i⟧ := by
   induction R generalizing Γ with
   | nil => exact i.elim0
   | cons _ _ I =>
@@ -34,6 +80,9 @@ theorem Eqv.inj_n_def {Γ : Ctx α ε} {R : LCtx α} {i : Fin R.length}
       apply congrArg
       ext
       simp [Term.inj_n, Term.inj, Term.Wf.inj_n, -Function.iterate_succ, Function.iterate_succ']
+
+theorem Eqv.inj_n_def' {Γ : Ctx α ε} {R : LCtx α} {i : Fin R.length}
+  : Eqv.inj_n (φ := φ) (Γ := Γ) (e := e) R i = nil.inj := by rw [inj_n_def, nil, var, inj_quot]; rfl
 
 -- def Eqv.pack_case {Γ : Ctx α ε} {R : LCtx α}
 --   (d : Eqv φ Γ (R.pack, e)) (G : ∀i : Fin R.length, Eqv φ ((R.get i, ⊥)::Γ) (A, e))
